proof/agp32_EX_CorrectScript.sml
@@ -7,287 +7,6 @@ val _ = prefer_num ();
 val _ = guess_lengths ();
 
 
-(* MARK: keep it here for EX proof later
-(* tactic *)
-val update_carry_flag_when_enabled_tac =
-    (Q.ABBREV_TAC `s = agp32 fext fbits t` >>
-     Q.ABBREV_TAC `s' = procs [agp32_next_state;WB_pipeline;MEM_pipeline;EX_pipeline;
-                               REG_write;ID_pipeline;IF_PC_update;Acc_compute]
-                              (fext t) s s` >>
-     Q.ABBREV_TAC `s'' = procs [ForwardA;ForwardB;ForwardW;IF_instr_update;
-                                ID_opc_func_update;ID_imm_update;
-                                ID_data_update;EX_ctrl_update;EX_forward_data;
-                                EX_ALU_input_update;EX_compute_enable_update]
-                               (fext (SUC t)) s' s'` >>                        
-     `(agp32 fext fbits (SUC t)).EX.EX_carry_flag =
-     (EX_ALU_update (fext (SUC t)) s' s'').EX.EX_carry_flag`
-       by fs [agp32_EX_ALU_items_updated_by_EX_ALU_update,Abbr `s`,Abbr `s'`,Abbr `s''`] >> rw []);
-
-val carry_flag_unchanged_tac =
-    (Q.ABBREV_TAC `s3 = procs [agp32_next_state;WB_pipeline;MEM_pipeline] (fext t) s s` >>
-     `?s4.(agp32 fext fbits (SUC t)).EX.EX_opc = (EX_pipeline (fext (SUC t)) s4 s3).EX.EX_opc`
-       by fs [agp32_EX_opc_func_updated_by_EX_pipeline,Abbr `s3`,Abbr `s`] >>
-     `(s3.ID.ID_EX_write_enable <=> s.ID.ID_EX_write_enable) /\ (s3.ID.ID_opc = s.ID.ID_opc)`
-       by METIS_TAC [Abbr `s3`,Abbr `s`,agp32_same_items_until_MEM_pipeline] >>
-     `s3.ID.ID_EX_write_enable` by fs [enable_stg_def] >>
-      Cases_on `enable_stg 2 s` >-
-      ((** ID is enabled at cycle t **)
-       `s.ID.ID_opc = opc ai` by (fs [Rel_def] >> `2 = 3 - 1 /\ 3 <> 1` by rw [] >>
-                              `I' (3,SUC t) = I' (2,t)` by METIS_TAC [Abbr `s`] >>
-                              fs [ID_Rel_def]) >>
-       `((agp32 fext fbits (SUC t)).EX.EX_opc = 16w) \/
-       ((agp32 fext fbits (SUC t)).EX.EX_opc = s.ID.ID_opc)`
-         by (fs [EX_pipeline_def] >> Cases_on `s3.EX.EX_NOP_flag` >> fs []) >>
-       `(s''.EX.EX_opc = (agp32 fext fbits (SUC t)).EX.EX_opc) /\
-       (s''.EX.EX_func = (agp32 fext fbits (SUC t)).EX.EX_func)`
-         by METIS_TAC [agp32_same_EX_opc_func_until_ALU_update,Abbr `s`,Abbr `s'`,Abbr `s''`] >>
-       `(s''.EX.EX_func = 9w) \/ (s''.EX.EX_func = 12w) \/ (s''.EX.EX_func = 13w) \/
-       (s''.EX.EX_func = 14w) \/ (s''.EX.EX_func = 15w)`
-         by fs [Abbr `s`,agp32_EX_opc_implies_EX_func] >>
-       `s''.EX.EX_carry_flag <=> s.EX.EX_carry_flag`
-         by METIS_TAC [agp32_same_EX_carry_flag_as_before,Abbr `s`,Abbr `s'`,Abbr `s''`] >>
-       rw [EX_ALU_update_def] >> fs [Rel_def,Abbr `s`]) >>
-     (** ID is disabled at cycle t **)
-     `s.EX.EX_NOP_flag` by fs [Abbr `s`,agp32_ID_enable_flags_imply_flush_NOP_flags,enable_stg_def] >>
-     `s3.EX.EX_NOP_flag <=> s.EX.EX_NOP_flag` by METIS_TAC [Abbr `s3`,Abbr `s`,agp32_same_items_until_MEM_pipeline] >>
-     fs [EX_pipeline_def] >>
-     `(s''.EX.EX_opc = (agp32 fext fbits (SUC t)).EX.EX_opc) /\
-     (s''.EX.EX_func = (agp32 fext fbits (SUC t)).EX.EX_func)`
-       by METIS_TAC [agp32_same_EX_opc_func_until_ALU_update,Abbr `s`,Abbr `s'`,Abbr `s''`] >>
-     `(s''.EX.EX_func = 9w) \/ (s''.EX.EX_func = 12w) \/ (s''.EX.EX_func = 13w) \/
-     (s''.EX.EX_func = 14w) \/ (s''.EX.EX_func = 15w)`
-       by fs [Abbr `s`,agp32_EX_opc_implies_EX_func] >>
-     `s''.EX.EX_carry_flag <=> s.EX.EX_carry_flag`
-       by METIS_TAC [agp32_same_EX_carry_flag_as_before,Abbr `s`,Abbr `s'`,Abbr `s''`] >>    
-     rw [EX_ALU_update_def] >> fs [Rel_def,Abbr `s`]);
-
-val carry_flag_unchanged_by_func_tac =
-    (Q.ABBREV_TAC `s3 = procs [agp32_next_state;WB_pipeline;MEM_pipeline] (fext t) s s` >>
-     `?s4.(agp32 fext fbits (SUC t)).EX.EX_func = (EX_pipeline (fext (SUC t)) s4 s3).EX.EX_func`
-       by fs [agp32_EX_opc_func_updated_by_EX_pipeline,Abbr `s3`,Abbr `s`] >>
-     `(s3.ID.ID_EX_write_enable <=> s.ID.ID_EX_write_enable) /\ (s3.ID.ID_func = s.ID.ID_func)`
-       by METIS_TAC [Abbr `s3`,Abbr `s`,agp32_same_items_until_MEM_pipeline] >>
-     `s3.ID.ID_EX_write_enable` by fs [enable_stg_def] >>
-      Cases_on `enable_stg 2 s` >-
-      ((** ID is enabled at cycle t **)
-       `s.ID.ID_func = func ai` by (fs [Rel_def] >> `2 = 3 - 1 /\ 3 <> 1` by rw [] >>
-                                    `I' (3,SUC t) = I' (2,t)` by METIS_TAC [Abbr `s`] >>
-                                    fs [ID_Rel_def]) >>
-       `((agp32 fext fbits (SUC t)).EX.EX_func = 12w) \/
-       ((agp32 fext fbits (SUC t)).EX.EX_func = s.ID.ID_func)`
-         by (fs [EX_pipeline_def] >> Cases_on `s3.EX.EX_NOP_flag` >> fs []) >>
-       `s''.EX.EX_func = (agp32 fext fbits (SUC t)).EX.EX_func`
-         by METIS_TAC [agp32_same_EX_opc_func_until_ALU_update,Abbr `s`,Abbr `s'`,Abbr `s''`] >>
-       `(s''.EX.EX_func <> 0w) /\ (s''.EX.EX_func <> 1w)` by fs [] >>
-       `s''.EX.EX_carry_flag <=> s.EX.EX_carry_flag`
-         by METIS_TAC [agp32_same_EX_carry_flag_as_before,Abbr `s`,Abbr `s'`,Abbr `s''`] >>
-       rw [EX_ALU_update_def] >> fs [Rel_def,Abbr `s`] >>
-       Cases_on_word_value `func ai` >> fs []) >>
-     (** ID is disabled at cycle t **)
-     `s.EX.EX_NOP_flag` by fs [Abbr `s`,agp32_ID_enable_flags_imply_flush_NOP_flags,enable_stg_def] >>
-     `s3.EX.EX_NOP_flag <=> s.EX.EX_NOP_flag` by METIS_TAC [Abbr `s3`,Abbr `s`,agp32_same_items_until_MEM_pipeline] >>
-     fs [EX_pipeline_def] >>
-     `s''.EX.EX_func = (agp32 fext fbits (SUC t)).EX.EX_func`
-       by METIS_TAC [agp32_same_EX_opc_func_until_ALU_update,Abbr `s`,Abbr `s'`,Abbr `s''`] >>
-     `s''.EX.EX_carry_flag <=> s.EX.EX_carry_flag`
-       by METIS_TAC [agp32_same_EX_carry_flag_as_before,Abbr `s`,Abbr `s'`,Abbr `s''`] >>    
-     rw [EX_ALU_update_def] >> fs [Rel_def,Abbr `s`]);
-
-(* lemmas *)
-(** lemmas copied from the hardware/ag32 repo **)
-
-(** copy end **)
-                                              
-
-
-(* carry_flag between ISA and circuit states *)
-Theorem agp32_Rel_ag32_carry_flag_correct:
-  !fext fbits a t I.
-    (!t k. enable_stg k (agp32 fext fbits t) ==> k <> 1 ==>
-           (I (k,SUC t) = I (k,t) + 1) /\ (I (k,SUC t) = I (k - 1,t))) ==>
-    (!t k. ~enable_stg k (agp32 fext fbits t) ==> I (k,SUC t) = I (k,t)) ==>
-    Rel I (fext t) (agp32 fext fbits (t-1)) (agp32 fext fbits t) a t ==>
-    ((agp32 fext fbits (SUC t)).EX.EX_carry_flag <=>
-     (FUNPOW Next (I (3,SUC t)) a).CarryFlag)
-Proof
-  rw [] >> Cases_on `enable_stg 3 (agp32 fext fbits t)` >-
-   (** EX stage is enabled **)
-   (`I'(3,SUC t) = SUC (I'(3,t))` by fs [] >>
-    rw [FUNPOW_SUC] >>
-    Q.ABBREV_TAC `ai = FUNPOW Next (I' (3,t)) a` >>             
-    rw [Next_def,GSYM word_at_addr_def,GSYM align_addr_def] >>
-    Cases_on `Decode (word_at_addr ai.MEM (align_addr ai.PC))` >-
-
-     ((** Accelerator **)
-     PairCases_on `p` >> rw [Run_def,dfn'Accelerator_def,incPC_def] >>
-     update_carry_flag_when_enabled_tac >>
-     `opc ai = 8w` by fs [ag32_Decode_Acc_opc_8w] >>
-     carry_flag_unchanged_tac) >-   
-
-     ((** In **)
-     rw [Run_def,dfn'In_def,incPC_def] >>
-     update_carry_flag_when_enabled_tac >>
-     `opc ai = 7w` by fs [ag32_Decode_In_opc_7w] >>
-     carry_flag_unchanged_tac) >-
-
-     ((** Interrupt **)
-     rw [Run_def,dfn'Interrupt_def,incPC_def] >>
-     update_carry_flag_when_enabled_tac >>
-     `opc ai = 12w` by fs [ag32_Decode_Interrupt_opc_12w] >>
-     carry_flag_unchanged_tac) >-
-
-     ((** Jump: CarryFlag can be changed **)
-     PairCases_on `p` >> rw [Run_def,dfn'Jump_def] >>
-     pairarg_tac >> fs [] >>
-     Cases_on `p0 = fAdd` >-
-      ((** fAdd **)
-      fs [ALU_def] >> rw [] >>
-      update_carry_flag_when_enabled_tac >>
-      `func ai = 0w` by fs [ag32_Decode_Jump_fAdd_func_0w] >>
-      `s''.EX.EX_func = 0w` by cheat >>
-      `s''.EX.EX_compute_enable` by cheat >>
-      rw [EX_ALU_update_def,ALU_correct_carry_lem,WORD_LS,word_add_def,w2n_w2w] >>
-      `(s''.EX.EX_ALU_input1 = ai.PC) /\ (s''.EX.EX_ALU_input2 = ri2word p2 ai)` by cheat >>
-      rw [] >> METIS_TAC [w2n_add_MOD_itself]) >>
-     Cases_on `p0 = fAddWithCarry` >-
-      ((** fAddWithCarry **)
-      fs [ALU_def] >> rw [] >>
-      cheat) >>
-     `s.CarryFlag = ai.CarryFlag` by (fs [ALU_def] >> Cases_on `p0` >> fs [] >> rw []) >>
-     fs [] >> rename1 `(v,ai')` >>
-     update_carry_flag_when_enabled_tac >>
-     `(func ai <> 0w) /\ (func ai <> 1w)` by fs [ag32_Decode_Jump_func_not_0w_1w] >>
-     carry_flag_unchanged_by_func_tac) >-
-
-     ((** JumpIfNotZero: CarryFlag can be changed **)
-     PairCases_on `p` >> rw [Run_def,dfn'JumpIfNotZero_def] >>
-     pairarg_tac >> fs [] >>
-     Cases_on `p0 = fAdd` >-
-      ((** fAdd **)
-      fs [ALU_def,incPC_def] >> rw [] >>
-      cheat) >>
-     Cases_on `p0 = fAddWithCarry` >-
-      ((** fAddWithCarry **)
-      fs [ALU_def,incPC_def] >> rw [] >>
-      cheat) >>
-     `s.CarryFlag = ai.CarryFlag` by (fs [ALU_def] >> Cases_on `p0` >> fs [] >> rw []) >>
-     fs [] >> rename1 `(v,ai')` >>
-     update_carry_flag_when_enabled_tac >> rw [incPC_def] >>
-     `(func ai <> 0w) /\ (func ai <> 1w)` by fs [ag32_Decode_JumpIfNotZero_func_not_0w_1w] >>
-     carry_flag_unchanged_by_func_tac) >-
-
-     ((** JumpIfZreo: CarryFlag can be changed **)
-     PairCases_on `p` >> rw [Run_def,dfn'JumpIfZero_def] >>
-     pairarg_tac >> fs [] >>
-     Cases_on `p0 = fAdd` >-
-      ((** fAdd **)
-      fs [ALU_def,incPC_def] >> rw [] >>
-      cheat) >>
-     Cases_on `p0 = fAddWithCarry` >-
-      ((** fAddWithCarry **)
-      fs [ALU_def,incPC_def] >> rw [] >>
-      cheat) >>
-     `s.CarryFlag = ai.CarryFlag` by (fs [ALU_def] >> Cases_on `p0` >> fs [] >> rw []) >>
-     fs [] >> rename1 `(v,ai')` >>
-     update_carry_flag_when_enabled_tac >> rw [incPC_def] >>
-     `(func ai <> 0w) /\ (func ai <> 1w)` by fs [ag32_Decode_JumpIfZero_func_not_0w_1w] >>
-     carry_flag_unchanged_by_func_tac) >-
-
-     ((** LoadConstant **)
-     PairCases_on `p` >> rw [Run_def,dfn'LoadConstant_def,incPC_def] >>
-     update_carry_flag_when_enabled_tac >>
-     `opc ai = 13w` by fs [ag32_Decode_LoadConstant_opc_13w] >>
-     carry_flag_unchanged_tac) >-
-
-     ((** LoadMEM **)
-     PairCases_on `p` >> rw [Run_def,dfn'LoadMEM_def,incPC_def] >>
-     update_carry_flag_when_enabled_tac >>
-     `opc ai = 4w` by fs [ag32_Decode_LoadMEM_opc_4w] >>
-     carry_flag_unchanged_tac) >-
-
-     ((** LoadMEMByte **)
-     PairCases_on `p` >> rw [Run_def,dfn'LoadMEMByte_def,incPC_def] >>
-     update_carry_flag_when_enabled_tac >>
-     `opc ai = 5w` by fs [ag32_Decode_LoadMEMByte_opc_5w] >>
-     carry_flag_unchanged_tac) >-
-
-     ((** LoadUpperConstant **)
-     PairCases_on `p` >> rw [Run_def,dfn'LoadUpperConstant_def,incPC_def] >>
-     update_carry_flag_when_enabled_tac >>
-     `opc ai = 14w` by fs [ag32_Decode_LoadUpperConstant_opc_14w] >>
-     carry_flag_unchanged_tac) >-
-
-     ((** Normal: CarryFlag can be changed **)
-     PairCases_on `p` >> rw [Run_def,dfn'Normal_def,norm_def,incPC_def] >>
-     pairarg_tac >> fs [] >>
-     Cases_on `p0 = fAdd` >-
-      ((** fAdd **)
-      fs [ALU_def] >> rw [] >>
-      cheat) >>
-     Cases_on `p0 = fAddWithCarry` >-         
-      ((** fAddWithCarry **)
-      fs [ALU_def] >> rw [] >>
-      cheat) >>
-     `s.CarryFlag = ai.CarryFlag` by (fs [ALU_def] >> Cases_on `p0` >> fs [] >> rw []) >>
-     fs [] >> rename1 `(v,ai')` >>
-     update_carry_flag_when_enabled_tac >>
-     `(func ai <> 0w) /\ (func ai <> 1w)` by fs [ag32_Decode_Normal_func_not_0w_1w] >>
-     carry_flag_unchanged_by_func_tac) >-
-
-     ((** Out: CarryFlag can be changed **)
-     PairCases_on `p` >> rw [Run_def,dfn'Out_def,norm_def,incPC_def] >>
-     pairarg_tac >> fs [] >>
-     Cases_on `p0 = fAdd` >-
-      ((** fAdd **)
-      fs [ALU_def] >> rw [] >>
-      cheat) >>
-     Cases_on `p0 = fAddWithCarry` >-         
-      ((** fAddWithCarry **)
-      fs [ALU_def] >> rw [] >>
-      cheat) >>
-     `s.CarryFlag = ai.CarryFlag` by (fs [ALU_def] >> Cases_on `p0` >> fs [] >> rw []) >>
-     fs [] >> rename1 `(v,ai')` >>
-     update_carry_flag_when_enabled_tac >>
-     `(func ai <> 0w) /\ (func ai <> 1w)` by fs [ag32_Decode_Out_func_not_0w_1w] >>
-     carry_flag_unchanged_by_func_tac) >-
-
-     ((** ReservedInstr **)
-     rw [Run_def] >>
-     update_carry_flag_when_enabled_tac >>
-     `opc ai = 15w` by fs [ag32_Decode_ReservedInstr_opc_15w] >>
-     carry_flag_unchanged_tac) >-
-
-     ((** Shift **)
-     PairCases_on `p` >> rw [Run_def,dfn'Shift_def,incPC_def] >>
-     update_carry_flag_when_enabled_tac >>
-     `opc ai = 1w` by fs [ag32_Decode_Shift_opc_1w] >>
-     carry_flag_unchanged_tac) >-
-
-     ((** StoreMEM **)
-     PairCases_on `p` >> rw [Run_def,dfn'StoreMEM_def,incPC_def] >>
-     update_carry_flag_when_enabled_tac >>
-     `opc ai = 2w` by fs [ag32_Decode_StoreMEM_opc_2w] >>
-     carry_flag_unchanged_tac) >>
-
-    (** StoreMEMByte **)
-    PairCases_on `p` >> rw [Run_def,dfn'StoreMEMByte_def,incPC_def] >>
-    update_carry_flag_when_enabled_tac >>
-    `opc ai = 3w` by fs [ag32_Decode_StoreMEMByte_opc_3w] >>
-    carry_flag_unchanged_tac) >>
-
-  (** EX stage is disabled **)
-  `I' (3,SUC t) = I' (3,t)` by fs [] >>
-  fs [Rel_def] >>
-  update_carry_flag_when_enabled_tac >>
-  reverse (Cases_on `s''.EX.EX_compute_enable`) >-
-   (`s''.EX.EX_carry_flag <=> s.EX.EX_carry_flag`
-      by METIS_TAC [agp32_same_EX_carry_flag_as_before,Abbr `s`,Abbr `s'`,Abbr `s''`] >>
-    fs [EX_ALU_update_def]) >>
-  cheat
-QED
- *)
-
-
 (** lemmas about words for ALU **)
 Theorem ALU_correct_carry_lem:
   !(w:33 word). word_bit 32 w <=> n2w (dimword(:32)) <=+ w
@@ -305,6 +24,24 @@ Theorem ALU_correct_v2w_carry32_lem:
   !b. v2w [b] = if b then (1w:32 word) else 0w
 Proof
   Cases >> EVAL_TAC
+QED
+
+Theorem w2n_add_MOD_itself:
+  !(w1:word32) (w2:word32).
+    w2n w1 + w2n w2 = (w2n w1 + w2n w2) MOD 8589934592
+Proof
+  rw [] >>
+  `(w2n w1 < 4294967296) /\ (w2n w2 < 4294967296)` by METIS_TAC [w2n_lt,dimword_32] >>
+  fs []
+QED
+
+Theorem w2n_add_MOD_itself_1:
+  !(w1:word32) (w2:word32).
+    w2n w1 + (w2n w2 + 1) = (w2n w1 + (w2n w2 + 1)) MOD 8589934592
+Proof
+  rw [] >>
+  `(w2n w1 < 4294967296) /\ (w2n w2 < 4294967296)` by METIS_TAC [w2n_lt,dimword_32] >>
+  fs []
 QED
 
 
@@ -773,10 +510,13 @@ Proof
   `(s''.ID.ID_EX_write_enable = s.ID.ID_EX_write_enable) /\
   (s''.EX.EX_overflow_flag = s.EX.EX_overflow_flag) /\
   (s''.EX.EX_carry_flag = s.EX.EX_carry_flag) /\
-  (s''.EX.EX_ALU_res = s.EX.EX_ALU_res)` by cheat >>
+  (s''.EX.EX_ALU_res = s.EX.EX_ALU_res)`
+    by METIS_TAC [agp32_same_items_until_EX_ALU_update,Abbr `s`,Abbr `s'`,Abbr `s''`] >>
   `(s''.EX.EX_ALU_input1 = (agp32 fext fbits (SUC t)).EX.EX_ALU_input1) /\
   (s''.EX.EX_ALU_input2 = (agp32 fext fbits (SUC t)).EX.EX_ALU_input2) /\
-  (s''.EX.EX_func = (agp32 fext fbits (SUC t)).EX.EX_func)` by cheat >>
+  (s''.EX.EX_func = (agp32 fext fbits (SUC t)).EX.EX_func)`
+    by METIS_TAC [agp32_same_EX_ALU_input_until_ALU_update,agp32_same_EX_opc_func_until_ALU_update,
+                  Abbr `s`,Abbr `s'`,Abbr `s''`] >>
   Cases_on `enable_stg 3 (agp32 fext fbits t)` >-
    (`s''.ID.ID_EX_write_enable` by fs [enable_stg_def,Abbr `s`] >>
     `s''.EX.EX_func = func (FUNPOW Next (THE (I' (3,SUC t)) − 1) a)`
@@ -792,13 +532,33 @@ Proof
        (fs [Rel_def] >>
         `THE (I' (3,SUC t)) = THE (I' (3,t)) + 1`
           by METIS_TAC [EX_instr_index_t_SUC_t_enable] >> fs []) >>
-      fs [] >> cheat) >-
+      fs [is_sch_def,is_sch_execute_def] >>
+      Cases_on `isJump_hw_op (agp32 fext fbits t)` >-
+       METIS_TAC [] >>
+      Cases_on `reg_data_hazard (agp32 fext fbits t)` >-
+       METIS_TAC [] >>
+      `I' (3,SUC t) = I' (2,t)` by fs [] >> fs [Rel_def]) >-
      (Cases_on `I' (3,t) <> NONE` >-
        (fs [Rel_def] >>
         `THE (I' (3,SUC t)) = THE (I' (3,t)) + 1`
           by METIS_TAC [EX_instr_index_t_SUC_t_enable] >> fs []) >>
-      fs [] >> cheat) >-
-     (`s.EX.EX_carry_flag = (FUNPOW Next (THE (I' (3,SUC t)) − 1) a).CarryFlag` by cheat >>
+      fs [is_sch_def,is_sch_execute_def] >>
+      Cases_on `isJump_hw_op (agp32 fext fbits t)` >-
+       METIS_TAC [] >>
+      Cases_on `reg_data_hazard (agp32 fext fbits t)` >-
+       METIS_TAC [] >>
+      `I' (3,SUC t) = I' (2,t)` by fs [] >> fs [Rel_def]) >-
+     (subgoal `s.EX.EX_carry_flag = (FUNPOW Next (THE (I' (3,SUC t)) − 1) a).CarryFlag` >-
+       (Cases_on `I' (3,t) <> NONE` >-
+         (fs [Rel_def] >>
+          `THE (I' (3,SUC t)) = THE (I' (3,t)) + 1`
+            by METIS_TAC [EX_instr_index_t_SUC_t_enable] >> fs []) >>
+        fs [is_sch_def,is_sch_execute_def] >>
+        Cases_on `isJump_hw_op (agp32 fext fbits t)` >-
+         METIS_TAC [] >>
+        Cases_on `reg_data_hazard (agp32 fext fbits t)` >-
+         METIS_TAC [] >>
+        `I' (3,SUC t) = I' (2,t)` by fs [] >> fs [Rel_def]) >>
       rw [ALU_correct_v2w_carry33_lem,ALU_correct_v2w_carry32_lem] >>
       BBLAST_TAC) >>
     BBLAST_TAC) >>
@@ -812,21 +572,529 @@ QED
 (* EX stage *)
 Theorem agp32_Rel_ag32_EX_Rel_correct:
   !fext fbits a t I.
-    is_sch_execute I (agp32 fext fbits) a ==>
-    is_sch_disable I (agp32 fext fbits) ==>
+    is_sch I (agp32 fext fbits) a ==>
     Rel I (fext t) (agp32 fext fbits (t-1)) (agp32 fext fbits t) a t ==>
     I (3,SUC t) <> NONE ==>
     EX_Rel (fext (SUC t)) (agp32 fext fbits (SUC t)) a (THE (I (3,SUC t)))
 Proof
   rw [EX_Rel_def] >>
-  fs [agp32_Rel_ag32_EX_PC_correct,agp32_Rel_ag32_EX_addrW_correct,
+  fs [is_sch_def,agp32_Rel_ag32_EX_PC_correct,agp32_Rel_ag32_EX_addrW_correct,
       agp32_Rel_ag32_EX_imm_correct,agp32_Rel_ag32_EX_opc_correct,
       agp32_Rel_ag32_EX_func_correct,agp32_Rel_ag32_EX_write_reg_correct,
       agp32_Rel_ag32_EX_dataA_correct,agp32_Rel_ag32_EX_dataB_correct,
       agp32_Rel_ag32_EX_dataW_correct,agp32_Rel_ag32_EX_imm_updated_correct_not_LoadUpperConstant,
       agp32_Rel_ag32_EX_imm_updated_correct_LoadUpperConstant,
-      agp32_Rel_ag32_EX_ALU_input1_correct,agp32_Rel_ag32_EX_ALU_input2_correct] >>
+      agp32_Rel_ag32_EX_ALU_input1_correct,agp32_Rel_ag32_EX_ALU_input2_correct,
+      agp32_Rel_ag32_EX_ALU_res_correct] >>
   cheat
+QED
+
+
+(** EX_ALU_carry_flag **)
+Theorem agp32_Rel_ag32_EX_ALU_carry_flag_correct:
+  !fext fbits a t I.
+    is_sch I (agp32 fext fbits) a ==>
+    Rel I (fext t) (agp32 fext fbits (t-1)) (agp32 fext fbits t) a t ==>
+    I (3,SUC t) <> NONE ==>
+    (agp32 fext fbits (SUC t)).EX.EX_carry_flag = (FUNPOW Next (THE (I (3,SUC t))) a).CarryFlag
+Proof
+  rw [] >> Q.ABBREV_TAC `s = agp32 fext fbits t` >>
+  Q.ABBREV_TAC `s' = procs [agp32_next_state;WB_pipeline;MEM_pipeline;EX_pipeline;
+                            REG_write;ID_pipeline;IF_PC_update;Acc_compute] (fext t) s s` >>
+  Q.ABBREV_TAC `s'' = procs [IF_instr_update;ID_opc_func_update;ID_imm_update;ID_data_update;
+                             ID_data_check_update;EX_ctrl_update;EX_ALU_input_imm_update] (fext (SUC t)) s' s'` >>
+  `(agp32 fext fbits (SUC t)).EX.EX_carry_flag = (EX_ALU_update (fext (SUC t)) s' s'').EX.EX_carry_flag`
+    by fs [agp32_EX_ALU_items_updated_by_EX_ALU_update] >>
+  `(s''.ID.ID_EX_write_enable = s.ID.ID_EX_write_enable) /\
+  (s''.EX.EX_overflow_flag = s.EX.EX_overflow_flag) /\
+  (s''.EX.EX_carry_flag = s.EX.EX_carry_flag) /\
+  (s''.EX.EX_ALU_res = s.EX.EX_ALU_res)`
+    by METIS_TAC [agp32_same_items_until_EX_ALU_update,Abbr `s`,Abbr `s'`,Abbr `s''`] >>
+  `(s''.EX.EX_ALU_input1 = (agp32 fext fbits (SUC t)).EX.EX_ALU_input1) /\
+  (s''.EX.EX_ALU_input2 = (agp32 fext fbits (SUC t)).EX.EX_ALU_input2) /\
+  (s''.EX.EX_func = (agp32 fext fbits (SUC t)).EX.EX_func) /\
+  (s''.EX.EX_opc = (agp32 fext fbits (SUC t)).EX.EX_opc)`
+    by METIS_TAC [agp32_same_EX_ALU_input_until_ALU_update,agp32_same_EX_opc_func_until_ALU_update,
+                  Abbr `s`,Abbr `s'`,Abbr `s''`] >>
+  Cases_on `enable_stg 3 (agp32 fext fbits t)` >-
+   (`s''.ID.ID_EX_write_enable` by fs [enable_stg_def,Abbr `s`] >>
+    `s''.EX.EX_func = func (FUNPOW Next (THE (I' (3,SUC t)) − 1) a)`
+      by fs [is_sch_def,agp32_Rel_ag32_EX_func_correct] >>
+    `s''.EX.EX_opc = opc (FUNPOW Next (THE (I' (3,SUC t)) − 1) a)`
+      by fs [is_sch_def,agp32_Rel_ag32_EX_opc_correct] >>
+    `s''.EX.EX_ALU_input1 = ALU_input1 (FUNPOW Next (THE (I' (3,SUC t)) − 1) a)`
+      by fs [is_sch_def,agp32_Rel_ag32_EX_ALU_input1_correct] >>
+    `s''.EX.EX_ALU_input2 = ALU_input2 (FUNPOW Next (THE (I' (3,SUC t)) − 1) a)`
+      by fs [is_sch_def,agp32_Rel_ag32_EX_ALU_input2_correct] >>
+    Cases_on `I' (3,t) <> NONE` >-
+     (`THE (I' (3,SUC t)) = SUC (THE (I' (3,t)))`
+        by METIS_TAC [EX_instr_index_t_SUC_t_enable,ADD1] >> fs [FUNPOW_SUC] >>
+      Q.ABBREV_TAC `ai = FUNPOW Next (THE (I' (3,t))) a` >>
+      rw [Next_def,GSYM word_at_addr_def,GSYM align_addr_def] >>
+      Cases_on `Decode (word_at_addr ai.MEM (align_addr ai.PC))` >-
+       (PairCases_on `p` >> rw [Run_def,dfn'Accelerator_def,incPC_def] >>
+        `opc ai = 8w` by fs [ag32_Decode_Acc_opc_8w] >>
+        `(s''.EX.EX_func = 9w) \/ (s''.EX.EX_func = 12w) \/ (s''.EX.EX_func = 13w) \/
+        (s''.EX.EX_func = 14w) \/ (s''.EX.EX_func = 15w)`
+          by fs [agp32_EX_opc_implies_EX_func] >>
+        fs [EX_ALU_update_def,Rel_def]) >-
+       (rw [Run_def,dfn'In_def,incPC_def] >>
+        `opc ai = 7w` by fs [ag32_Decode_In_opc_7w] >>
+        `(s''.EX.EX_func = 9w) \/ (s''.EX.EX_func = 12w) \/ (s''.EX.EX_func = 13w) \/
+        (s''.EX.EX_func = 14w) \/ (s''.EX.EX_func = 15w)`
+          by fs [agp32_EX_opc_implies_EX_func] >>
+        fs [EX_ALU_update_def,Rel_def]) >-
+       (rw [Run_def,dfn'Interrupt_def,incPC_def] >>
+        `opc ai = 12w` by fs [ag32_Decode_Interrupt_opc_12w] >>
+        `(s''.EX.EX_func = 9w) \/ (s''.EX.EX_func = 12w) \/ (s''.EX.EX_func = 13w) \/
+        (s''.EX.EX_func = 14w) \/ (s''.EX.EX_func = 15w)`
+          by fs [agp32_EX_opc_implies_EX_func] >>
+        fs [EX_ALU_update_def,Rel_def]) >-
+       (PairCases_on `p` >> rw [Run_def,dfn'Jump_def] >>
+        `opc ai = 9w` by fs [ag32_Decode_Jump_opc_9w] >>
+        pairarg_tac >> fs [] >>
+        Cases_on `p0 = fAdd` >-
+         (fs [ALU_def] >> rw [] >>
+          `func ai = 0w` by fs [ag32_Decode_Jump_fAdd_func_0w] >> fs [] >>
+          rw [EX_ALU_update_def,ALU_correct_carry_lem,WORD_LS,word_add_def,w2n_w2w] >>
+          fs [ALU_input1_def,ALU_input2_def] >>
+          `dataA ai = ri2word p2 ai` by fs [ag32_Decode_Jump_dataA] >>
+          rw [] >> METIS_TAC [w2n_add_MOD_itself]) >>
+        Cases_on `p0 = fAddWithCarry` >-
+         (fs [ALU_def] >> rw [] >>
+          `func ai = 1w` by fs [ag32_Decode_Jump_fAddWithCarry_func_1w] >> fs [] >>
+          rw [EX_ALU_update_def,ALU_correct_carry_lem,WORD_LS,word_add_def,w2n_w2w] >>
+          fs [ALU_input1_def,ALU_input2_def] >>
+          `dataA ai = ri2word p2 ai` by fs [ag32_Decode_Jump_dataA] >-
+           (`s.EX.EX_carry_flag` by fs [Rel_def] >>
+            rw [v2w_single_1w,ALU_correct_v2w_carry33_lem] >>
+            METIS_TAC [w2n_add_MOD_itself_1]) >>
+          `~s.EX.EX_carry_flag` by fs [Rel_def] >>
+          rw [v2w_single_0w,ALU_correct_v2w_carry33_lem] >>
+          METIS_TAC [w2n_add_MOD_itself]) >>
+        fs [] >> rename1 `(v,ai')` >>
+        `ai'.CarryFlag = ai.CarryFlag` by (fs [ALU_def] >> Cases_on `p0` >> fs [] >> rw []) >>
+        `(func ai <> 0w) /\ (func ai <> 1w)` by fs [ag32_Decode_Jump_func_not_0w_1w] >>
+        fs [EX_ALU_update_def,Rel_def] >>
+        Cases_on_word_value `(agp32 fext fbits (SUC t)).EX.EX_func` >> fs []) >-
+       (PairCases_on `p` >> rw [Run_def,dfn'JumpIfNotZero_def] >>
+        `opc ai = 11w` by fs [ag32_Decode_JumpIfNotZero_opc_11w] >>
+        pairarg_tac >> fs [] >>
+        Cases_on `p0 = fAdd` >-
+         (fs [ALU_def] >> rw [] >>
+          `func ai = 0w` by fs [ag32_Decode_JumpIfNotZero_fAdd_func_0w] >> fs [] >>
+          rw [EX_ALU_update_def,ALU_correct_carry_lem,WORD_LS,word_add_def,w2n_w2w] >>
+          fs [ALU_input1_def,ALU_input2_def] >>
+          `(dataA ai = ri2word p2 ai) /\ (dataB ai = ri2word p3 ai)`
+            by fs [ag32_Decode_JumpIfNotZero_dataA,ag32_Decode_JumpIfNotZero_dataB] >>
+          rw [incPC_def] >> METIS_TAC [w2n_add_MOD_itself]) >>
+        Cases_on `p0 = fAddWithCarry` >-
+         (fs [ALU_def] >> rw [] >>
+          `func ai = 1w` by fs [ag32_Decode_JumpIfNotZero_fAddWithCarry_func_1w] >> fs [] >>
+          rw [EX_ALU_update_def,ALU_correct_carry_lem,WORD_LS,word_add_def,w2n_w2w] >>
+          fs [ALU_input1_def,ALU_input2_def] >>
+          `(dataA ai = ri2word p2 ai) /\ (dataB ai = ri2word p3 ai)`
+            by fs [ag32_Decode_JumpIfNotZero_dataA,ag32_Decode_JumpIfNotZero_dataB] >-
+           (`s.EX.EX_carry_flag` by fs [Rel_def] >>
+            rw [v2w_single_1w,ALU_correct_v2w_carry33_lem] >>
+            METIS_TAC [w2n_add_MOD_itself_1]) >-
+           (`~s.EX.EX_carry_flag` by fs [Rel_def] >>
+            rw [v2w_single_0w,ALU_correct_v2w_carry33_lem] >>
+            METIS_TAC [w2n_add_MOD_itself]) >-
+           (`s.EX.EX_carry_flag` by fs [Rel_def] >>
+            rw [v2w_single_1w,ALU_correct_v2w_carry33_lem,incPC_def] >>
+            METIS_TAC [w2n_add_MOD_itself_1]) >>
+          `~s.EX.EX_carry_flag` by fs [Rel_def] >>
+          rw [v2w_single_0w,ALU_correct_v2w_carry33_lem,incPC_def] >>
+          METIS_TAC [w2n_add_MOD_itself]) >>
+        fs [] >> rename1 `(v,ai')` >>
+        `ai'.CarryFlag = ai.CarryFlag` by (fs [ALU_def] >> Cases_on `p0` >> fs [] >> rw []) >>
+        `(func ai <> 0w) /\ (func ai <> 1w)` by fs [ag32_Decode_JumpIfNotZero_func_not_0w_1w] >>
+        Cases_on `v` >> rw [incPC_def] >>
+        fs [EX_ALU_update_def,Rel_def,incPC_def] >>
+        Cases_on_word_value `(agp32 fext fbits (SUC t)).EX.EX_func` >> fs []) >-
+       (PairCases_on `p` >> rw [Run_def,dfn'JumpIfZero_def] >>
+        `opc ai = 10w` by fs [ag32_Decode_JumpIfZero_opc_10w] >>
+        pairarg_tac >> fs [] >>
+        Cases_on `p0 = fAdd` >-
+         (fs [ALU_def] >> rw [] >>
+          `func ai = 0w` by fs [ag32_Decode_JumpIfZero_fAdd_func_0w] >> fs [] >>
+          rw [EX_ALU_update_def,ALU_correct_carry_lem,WORD_LS,word_add_def,w2n_w2w] >>
+          fs [ALU_input1_def,ALU_input2_def] >>
+          `(dataA ai = ri2word p2 ai) /\ (dataB ai = ri2word p3 ai)`
+            by fs [ag32_Decode_JumpIfZero_dataA,ag32_Decode_JumpIfZero_dataB] >>
+          rw [incPC_def] >> METIS_TAC [w2n_add_MOD_itself]) >>
+        Cases_on `p0 = fAddWithCarry` >-
+         (fs [ALU_def] >> rw [] >>
+          `func ai = 1w` by fs [ag32_Decode_JumpIfZero_fAddWithCarry_func_1w] >> fs [] >>
+          rw [EX_ALU_update_def,ALU_correct_carry_lem,WORD_LS,word_add_def,w2n_w2w] >>
+          fs [ALU_input1_def,ALU_input2_def] >>
+          `(dataA ai = ri2word p2 ai) /\ (dataB ai = ri2word p3 ai)`
+            by fs [ag32_Decode_JumpIfZero_dataA,ag32_Decode_JumpIfZero_dataB] >-
+           (`s.EX.EX_carry_flag` by fs [Rel_def] >>
+            rw [v2w_single_1w,ALU_correct_v2w_carry33_lem] >>
+            METIS_TAC [w2n_add_MOD_itself_1]) >-
+           (`~s.EX.EX_carry_flag` by fs [Rel_def] >>
+            rw [v2w_single_0w,ALU_correct_v2w_carry33_lem] >>
+            METIS_TAC [w2n_add_MOD_itself]) >-
+           (`s.EX.EX_carry_flag` by fs [Rel_def] >>
+            rw [v2w_single_1w,ALU_correct_v2w_carry33_lem,incPC_def] >>
+            METIS_TAC [w2n_add_MOD_itself_1]) >>
+          `~s.EX.EX_carry_flag` by fs [Rel_def] >>
+          rw [v2w_single_0w,ALU_correct_v2w_carry33_lem,incPC_def] >>
+          METIS_TAC [w2n_add_MOD_itself]) >>
+        fs [] >> rename1 `(v,ai')` >>
+        `ai'.CarryFlag = ai.CarryFlag` by (fs [ALU_def] >> Cases_on `p0` >> fs [] >> rw []) >>
+        `(func ai <> 0w) /\ (func ai <> 1w)` by fs [ag32_Decode_JumpIfZero_func_not_0w_1w] >>
+        Cases_on `v` >> rw [incPC_def] >>
+        fs [EX_ALU_update_def,Rel_def,incPC_def] >>
+        Cases_on_word_value `(agp32 fext fbits (SUC t)).EX.EX_func` >> fs []) >-
+       (PairCases_on `p` >> rw [Run_def,dfn'LoadConstant_def,incPC_def] >>
+        `opc ai = 13w` by fs [ag32_Decode_LoadConstant_opc_13w] >>
+        `(s''.EX.EX_func = 9w) \/ (s''.EX.EX_func = 12w) \/ (s''.EX.EX_func = 13w) \/
+        (s''.EX.EX_func = 14w) \/ (s''.EX.EX_func = 15w)`
+          by fs [agp32_EX_opc_implies_EX_func] >>
+        fs [EX_ALU_update_def,Rel_def]) >-
+       (PairCases_on `p` >> rw [Run_def,dfn'LoadMEM_def,incPC_def] >>
+        `opc ai = 4w` by fs [ag32_Decode_LoadMEM_opc_4w] >>
+        `(s''.EX.EX_func = 9w) \/ (s''.EX.EX_func = 12w) \/ (s''.EX.EX_func = 13w) \/
+        (s''.EX.EX_func = 14w) \/ (s''.EX.EX_func = 15w)`
+          by fs [agp32_EX_opc_implies_EX_func] >>
+        fs [EX_ALU_update_def,Rel_def]) >-
+       (PairCases_on `p` >> rw [Run_def,dfn'LoadMEMByte_def,incPC_def] >>
+        `opc ai = 5w` by fs [ag32_Decode_LoadMEMByte_opc_5w] >>
+        `(s''.EX.EX_func = 9w) \/ (s''.EX.EX_func = 12w) \/ (s''.EX.EX_func = 13w) \/
+        (s''.EX.EX_func = 14w) \/ (s''.EX.EX_func = 15w)`
+          by fs [agp32_EX_opc_implies_EX_func] >>
+        fs [EX_ALU_update_def,Rel_def]) >-
+       (PairCases_on `p` >> rw [Run_def,dfn'LoadUpperConstant_def,incPC_def] >>
+        `opc ai = 14w` by fs [ag32_Decode_LoadUpperConstant_opc_14w] >>
+        `(s''.EX.EX_func = 9w) \/ (s''.EX.EX_func = 12w) \/ (s''.EX.EX_func = 13w) \/
+        (s''.EX.EX_func = 14w) \/ (s''.EX.EX_func = 15w)`
+          by fs [agp32_EX_opc_implies_EX_func] >>
+        fs [EX_ALU_update_def,Rel_def]) >-
+       (PairCases_on `p` >> rw [Run_def,dfn'Normal_def,norm_def,incPC_def] >>
+        `opc ai = 0w` by fs [ag32_Decode_Normal_opc_0w] >>
+        pairarg_tac >> fs [] >>
+        Cases_on `p0 = fAdd` >-
+         (fs [ALU_def] >> rw [] >>
+          `func ai = 0w` by fs [ag32_Decode_Normal_fAdd_func_0w] >> fs [] >>
+          rw [EX_ALU_update_def,ALU_correct_carry_lem,WORD_LS,word_add_def,w2n_w2w] >>
+          fs [ALU_input1_def,ALU_input2_def] >>
+          `(dataA ai = ri2word p2 ai) /\ (dataB ai = ri2word p3 ai)`
+            by fs [ag32_Decode_Normal_dataA,ag32_Decode_Normal_dataB] >>
+          rw [] >> METIS_TAC [w2n_add_MOD_itself]) >>
+        Cases_on `p0 = fAddWithCarry` >-
+         (fs [ALU_def] >> rw [] >>
+          `func ai = 1w` by fs [ag32_Decode_Normal_fAddWithCarry_func_1w] >> fs [] >>
+          rw [EX_ALU_update_def,ALU_correct_carry_lem,WORD_LS,word_add_def,w2n_w2w] >>
+          fs [ALU_input1_def,ALU_input2_def] >>
+          `(dataA ai = ri2word p2 ai) /\ (dataB ai = ri2word p3 ai)`
+            by fs [ag32_Decode_Normal_dataA,ag32_Decode_Normal_dataB] >-
+           (`s.EX.EX_carry_flag` by fs [Rel_def] >>
+            rw [v2w_single_1w,ALU_correct_v2w_carry33_lem] >>
+            METIS_TAC [w2n_add_MOD_itself_1]) >>
+          `~s.EX.EX_carry_flag` by fs [Rel_def] >>
+          rw [v2w_single_0w,ALU_correct_v2w_carry33_lem] >>
+          METIS_TAC [w2n_add_MOD_itself]) >>
+        fs [] >> rename1 `(v,ai')` >>
+        `ai'.CarryFlag = ai.CarryFlag` by (fs [ALU_def] >> Cases_on `p0` >> fs [] >> rw []) >>
+        `(func ai <> 0w) /\ (func ai <> 1w)` by fs [ag32_Decode_Normal_func_not_0w_1w] >>
+        fs [EX_ALU_update_def,Rel_def] >>
+        Cases_on_word_value `(agp32 fext fbits (SUC t)).EX.EX_func` >> fs []) >-
+       (PairCases_on `p` >> rw [Run_def,dfn'Out_def,norm_def,incPC_def] >>
+        `opc ai = 6w` by fs [ag32_Decode_Out_opc_6w] >>
+        pairarg_tac >> fs [] >>
+        Cases_on `p0 = fAdd` >-
+         (fs [ALU_def] >> rw [] >>
+          `func ai = 0w` by fs [ag32_Decode_Out_fAdd_func_0w] >> fs [] >>
+          rw [EX_ALU_update_def,ALU_correct_carry_lem,WORD_LS,word_add_def,w2n_w2w] >>
+          fs [ALU_input1_def,ALU_input2_def] >>
+          `(dataA ai = ri2word p2 ai) /\ (dataB ai = ri2word p3 ai)`
+            by fs [ag32_Decode_Out_dataA,ag32_Decode_Out_dataB] >>
+          rw [] >> METIS_TAC [w2n_add_MOD_itself]) >>
+        Cases_on `p0 = fAddWithCarry` >-
+         (fs [ALU_def] >> rw [] >>
+          `func ai = 1w` by fs [ag32_Decode_Out_fAddWithCarry_func_1w] >> fs [] >>
+          rw [EX_ALU_update_def,ALU_correct_carry_lem,WORD_LS,word_add_def,w2n_w2w] >>
+          fs [ALU_input1_def,ALU_input2_def] >>
+          `(dataA ai = ri2word p2 ai) /\ (dataB ai = ri2word p3 ai)`
+            by fs [ag32_Decode_Out_dataA,ag32_Decode_Out_dataB] >-
+           (`s.EX.EX_carry_flag` by fs [Rel_def] >>
+            rw [v2w_single_1w,ALU_correct_v2w_carry33_lem] >>
+            METIS_TAC [w2n_add_MOD_itself_1]) >>
+          `~s.EX.EX_carry_flag` by fs [Rel_def] >>
+          rw [v2w_single_0w,ALU_correct_v2w_carry33_lem] >>
+          METIS_TAC [w2n_add_MOD_itself]) >>
+        fs [] >> rename1 `(v,ai')` >>
+        `ai'.CarryFlag = ai.CarryFlag` by (fs [ALU_def] >> Cases_on `p0` >> fs [] >> rw []) >>
+        `(func ai <> 0w) /\ (func ai <> 1w)` by fs [ag32_Decode_Out_func_not_0w_1w] >>
+        fs [EX_ALU_update_def,Rel_def] >>
+        Cases_on_word_value `(agp32 fext fbits (SUC t)).EX.EX_func` >> fs []) >-
+       (rw [Run_def] >>
+        `opc ai = 15w` by fs [ag32_Decode_ReservedInstr_opc_15w] >>
+        `(s''.EX.EX_func = 9w) \/ (s''.EX.EX_func = 12w) \/ (s''.EX.EX_func = 13w) \/
+        (s''.EX.EX_func = 14w) \/ (s''.EX.EX_func = 15w)`
+          by fs [agp32_EX_opc_implies_EX_func] >>
+        fs [EX_ALU_update_def,Rel_def]) >-
+       (PairCases_on `p` >> rw [Run_def,dfn'Shift_def,incPC_def] >>
+        `opc ai = 1w` by fs [ag32_Decode_Shift_opc_1w] >>
+        `(s''.EX.EX_func = 9w) \/ (s''.EX.EX_func = 12w) \/ (s''.EX.EX_func = 13w) \/
+        (s''.EX.EX_func = 14w) \/ (s''.EX.EX_func = 15w)`
+          by fs [agp32_EX_opc_implies_EX_func] >>
+        fs [EX_ALU_update_def,Rel_def]) >-
+       (PairCases_on `p` >> rw [Run_def,dfn'StoreMEM_def,incPC_def] >>
+        `opc ai = 2w` by fs [ag32_Decode_StoreMEM_opc_2w] >>
+        `(s''.EX.EX_func = 9w) \/ (s''.EX.EX_func = 12w) \/ (s''.EX.EX_func = 13w) \/
+        (s''.EX.EX_func = 14w) \/ (s''.EX.EX_func = 15w)`
+          by fs [agp32_EX_opc_implies_EX_func] >>
+        fs [EX_ALU_update_def,Rel_def]) >>
+      PairCases_on `p` >> rw [Run_def,dfn'StoreMEMByte_def,incPC_def] >>
+      `opc ai = 3w` by fs [ag32_Decode_StoreMEMByte_opc_3w] >>
+      `(s''.EX.EX_func = 9w) \/ (s''.EX.EX_func = 12w) \/ (s''.EX.EX_func = 13w) \/
+      (s''.EX.EX_func = 14w) \/ (s''.EX.EX_func = 15w)`
+        by fs [agp32_EX_opc_implies_EX_func] >>
+      fs [EX_ALU_update_def,Rel_def]) >>
+    subgoal `I' (3,SUC t) = I' (2,t)` >-
+     (fs [is_sch_def,is_sch_execute_def] >>
+      Cases_on `isJump_hw_op (agp32 fext fbits t)` >>
+      Cases_on `reg_data_hazard (agp32 fext fbits t)` >>
+      METIS_TAC []) >> fs [] >>
+    `THE (I' (2,t)) = SUC (THE (I' (2,t)) - 1)`
+      by (Cases_on `THE (I' (2,t))` >- METIS_TAC [ID_instr_index_not_0] >> fs []) >>
+    `(FUNPOW Next (THE (I' (2,t))) a).CarryFlag =
+    (FUNPOW Next (SUC (THE (I' (2,t)) - 1)) a).CarryFlag` by METIS_TAC [] >>       
+    fs [FUNPOW_SUC] >>
+    Q.ABBREV_TAC `ai = FUNPOW Next (THE (I' (2,t)) - 1) a` >>
+    rw [Next_def,GSYM word_at_addr_def,GSYM align_addr_def] >>
+    Cases_on `Decode (word_at_addr ai.MEM (align_addr ai.PC))` >-
+     (PairCases_on `p` >> rw [Run_def,dfn'Accelerator_def,incPC_def] >>
+      `opc ai = 8w` by fs [ag32_Decode_Acc_opc_8w] >>
+      `(s''.EX.EX_func = 9w) \/ (s''.EX.EX_func = 12w) \/ (s''.EX.EX_func = 13w) \/
+      (s''.EX.EX_func = 14w) \/ (s''.EX.EX_func = 15w)`         
+        by fs [agp32_EX_opc_implies_EX_func] >>
+      fs [EX_ALU_update_def,Rel_def]) >-
+     (rw [Run_def,dfn'In_def,incPC_def] >>
+      `opc ai = 7w` by fs [ag32_Decode_In_opc_7w] >>
+      `(s''.EX.EX_func = 9w) \/ (s''.EX.EX_func = 12w) \/ (s''.EX.EX_func = 13w) \/
+      (s''.EX.EX_func = 14w) \/ (s''.EX.EX_func = 15w)`
+        by fs [agp32_EX_opc_implies_EX_func] >>
+      fs [EX_ALU_update_def,Rel_def]) >-
+     (rw [Run_def,dfn'Interrupt_def,incPC_def] >>
+      `opc ai = 12w` by fs [ag32_Decode_Interrupt_opc_12w] >>
+      `(s''.EX.EX_func = 9w) \/ (s''.EX.EX_func = 12w) \/ (s''.EX.EX_func = 13w) \/
+      (s''.EX.EX_func = 14w) \/ (s''.EX.EX_func = 15w)`
+        by fs [agp32_EX_opc_implies_EX_func] >>
+      fs [EX_ALU_update_def,Rel_def]) >-
+     (PairCases_on `p` >> rw [Run_def,dfn'Jump_def] >>
+      `opc ai = 9w` by fs [ag32_Decode_Jump_opc_9w] >>
+      pairarg_tac >> fs [] >>
+      Cases_on `p0 = fAdd` >-
+       (fs [ALU_def] >> rw [] >>
+        `func ai = 0w` by fs [ag32_Decode_Jump_fAdd_func_0w] >> fs [] >>
+        rw [EX_ALU_update_def,ALU_correct_carry_lem,WORD_LS,word_add_def,w2n_w2w] >>
+        fs [ALU_input1_def,ALU_input2_def] >>
+        `dataA ai = ri2word p2 ai` by fs [ag32_Decode_Jump_dataA] >>
+        rw [] >> METIS_TAC [w2n_add_MOD_itself]) >>
+      Cases_on `p0 = fAddWithCarry` >-
+       (fs [ALU_def] >> rw [] >>
+        `func ai = 1w` by fs [ag32_Decode_Jump_fAddWithCarry_func_1w] >> fs [] >>
+        rw [EX_ALU_update_def,ALU_correct_carry_lem,WORD_LS,word_add_def,w2n_w2w] >>
+        fs [ALU_input1_def,ALU_input2_def] >>
+        `dataA ai = ri2word p2 ai` by fs [ag32_Decode_Jump_dataA] >-
+         (`s.EX.EX_carry_flag` by fs [Rel_def] >>
+          rw [v2w_single_1w,ALU_correct_v2w_carry33_lem] >>
+          METIS_TAC [w2n_add_MOD_itself_1]) >>
+        `~s.EX.EX_carry_flag` by fs [Rel_def] >>
+        rw [v2w_single_0w,ALU_correct_v2w_carry33_lem] >>
+        METIS_TAC [w2n_add_MOD_itself]) >>
+      fs [] >> rename1 `(v,ai')` >>
+      `ai'.CarryFlag = ai.CarryFlag` by (fs [ALU_def] >> Cases_on `p0` >> fs [] >> rw []) >>
+      `(func ai <> 0w) /\ (func ai <> 1w)` by fs [ag32_Decode_Jump_func_not_0w_1w] >>
+      fs [EX_ALU_update_def,Rel_def] >>
+      Cases_on_word_value `(agp32 fext fbits (SUC t)).EX.EX_func` >> fs []) >-
+     (PairCases_on `p` >> rw [Run_def,dfn'JumpIfNotZero_def] >>
+      `opc ai = 11w` by fs [ag32_Decode_JumpIfNotZero_opc_11w] >>
+      pairarg_tac >> fs [] >>
+      Cases_on `p0 = fAdd` >-
+       (fs [ALU_def] >> rw [] >>
+        `func ai = 0w` by fs [ag32_Decode_JumpIfNotZero_fAdd_func_0w] >> fs [] >>
+        rw [EX_ALU_update_def,ALU_correct_carry_lem,WORD_LS,word_add_def,w2n_w2w] >>
+        fs [ALU_input1_def,ALU_input2_def] >>
+        `(dataA ai = ri2word p2 ai) /\ (dataB ai = ri2word p3 ai)`
+          by fs [ag32_Decode_JumpIfNotZero_dataA,ag32_Decode_JumpIfNotZero_dataB] >>
+        rw [incPC_def] >> METIS_TAC [w2n_add_MOD_itself]) >>
+      Cases_on `p0 = fAddWithCarry` >-
+       (fs [ALU_def] >> rw [] >>
+        `func ai = 1w` by fs [ag32_Decode_JumpIfNotZero_fAddWithCarry_func_1w] >> fs [] >>
+        rw [EX_ALU_update_def,ALU_correct_carry_lem,WORD_LS,word_add_def,w2n_w2w] >>
+        fs [ALU_input1_def,ALU_input2_def] >>
+        `(dataA ai = ri2word p2 ai) /\ (dataB ai = ri2word p3 ai)`
+          by fs [ag32_Decode_JumpIfNotZero_dataA,ag32_Decode_JumpIfNotZero_dataB] >-
+         (`s.EX.EX_carry_flag` by fs [Rel_def] >>
+          rw [v2w_single_1w,ALU_correct_v2w_carry33_lem] >>
+          METIS_TAC [w2n_add_MOD_itself_1]) >-
+         (`~s.EX.EX_carry_flag` by fs [Rel_def] >>
+          rw [v2w_single_0w,ALU_correct_v2w_carry33_lem] >>
+          METIS_TAC [w2n_add_MOD_itself]) >-
+         (`s.EX.EX_carry_flag` by fs [Rel_def] >>
+          rw [v2w_single_1w,ALU_correct_v2w_carry33_lem,incPC_def] >>
+          METIS_TAC [w2n_add_MOD_itself_1]) >>
+        `~s.EX.EX_carry_flag` by fs [Rel_def] >>
+        rw [v2w_single_0w,ALU_correct_v2w_carry33_lem,incPC_def] >>
+        METIS_TAC [w2n_add_MOD_itself]) >>
+      fs [] >> rename1 `(v,ai')` >>
+      `ai'.CarryFlag = ai.CarryFlag` by (fs [ALU_def] >> Cases_on `p0` >> fs [] >> rw []) >>
+      `(func ai <> 0w) /\ (func ai <> 1w)` by fs [ag32_Decode_JumpIfNotZero_func_not_0w_1w] >>
+      Cases_on `v` >> rw [incPC_def] >>
+      fs [EX_ALU_update_def,Rel_def,incPC_def] >>
+      Cases_on_word_value `(agp32 fext fbits (SUC t)).EX.EX_func` >> fs []) >-
+     (PairCases_on `p` >> rw [Run_def,dfn'JumpIfZero_def] >>
+      `opc ai = 10w` by fs [ag32_Decode_JumpIfZero_opc_10w] >>
+      pairarg_tac >> fs [] >>
+      Cases_on `p0 = fAdd` >-
+       (fs [ALU_def] >> rw [] >>
+        `func ai = 0w` by fs [ag32_Decode_JumpIfZero_fAdd_func_0w] >> fs [] >>
+        rw [EX_ALU_update_def,ALU_correct_carry_lem,WORD_LS,word_add_def,w2n_w2w] >>
+        fs [ALU_input1_def,ALU_input2_def] >>
+        `(dataA ai = ri2word p2 ai) /\ (dataB ai = ri2word p3 ai)`
+          by fs [ag32_Decode_JumpIfZero_dataA,ag32_Decode_JumpIfZero_dataB] >>
+        rw [incPC_def] >> METIS_TAC [w2n_add_MOD_itself]) >>
+      Cases_on `p0 = fAddWithCarry` >-
+       (fs [ALU_def] >> rw [] >>
+        `func ai = 1w` by fs [ag32_Decode_JumpIfZero_fAddWithCarry_func_1w] >> fs [] >>
+        rw [EX_ALU_update_def,ALU_correct_carry_lem,WORD_LS,word_add_def,w2n_w2w] >>
+        fs [ALU_input1_def,ALU_input2_def] >>
+        `(dataA ai = ri2word p2 ai) /\ (dataB ai = ri2word p3 ai)`
+          by fs [ag32_Decode_JumpIfZero_dataA,ag32_Decode_JumpIfZero_dataB] >-
+         (`s.EX.EX_carry_flag` by fs [Rel_def] >>
+          rw [v2w_single_1w,ALU_correct_v2w_carry33_lem] >>
+          METIS_TAC [w2n_add_MOD_itself_1]) >-
+         (`~s.EX.EX_carry_flag` by fs [Rel_def] >>
+          rw [v2w_single_0w,ALU_correct_v2w_carry33_lem] >>
+          METIS_TAC [w2n_add_MOD_itself]) >-
+         (`s.EX.EX_carry_flag` by fs [Rel_def] >>
+          rw [v2w_single_1w,ALU_correct_v2w_carry33_lem,incPC_def] >>
+          METIS_TAC [w2n_add_MOD_itself_1]) >>
+        `~s.EX.EX_carry_flag` by fs [Rel_def] >>
+        rw [v2w_single_0w,ALU_correct_v2w_carry33_lem,incPC_def] >>
+        METIS_TAC [w2n_add_MOD_itself]) >>
+      fs [] >> rename1 `(v,ai')` >>
+      `ai'.CarryFlag = ai.CarryFlag` by (fs [ALU_def] >> Cases_on `p0` >> fs [] >> rw []) >>
+      `(func ai <> 0w) /\ (func ai <> 1w)` by fs [ag32_Decode_JumpIfZero_func_not_0w_1w] >>
+      Cases_on `v` >> rw [incPC_def] >>
+      fs [EX_ALU_update_def,Rel_def,incPC_def] >>
+      Cases_on_word_value `(agp32 fext fbits (SUC t)).EX.EX_func` >> fs []) >-
+     (PairCases_on `p` >> rw [Run_def,dfn'LoadConstant_def,incPC_def] >>
+      `opc ai = 13w` by fs [ag32_Decode_LoadConstant_opc_13w] >>
+      `(s''.EX.EX_func = 9w) \/ (s''.EX.EX_func = 12w) \/ (s''.EX.EX_func = 13w) \/
+      (s''.EX.EX_func = 14w) \/ (s''.EX.EX_func = 15w)`
+        by fs [agp32_EX_opc_implies_EX_func] >>
+      fs [EX_ALU_update_def,Rel_def]) >-
+     (PairCases_on `p` >> rw [Run_def,dfn'LoadMEM_def,incPC_def] >>
+      `opc ai = 4w` by fs [ag32_Decode_LoadMEM_opc_4w] >>
+      `(s''.EX.EX_func = 9w) \/ (s''.EX.EX_func = 12w) \/ (s''.EX.EX_func = 13w) \/
+      (s''.EX.EX_func = 14w) \/ (s''.EX.EX_func = 15w)`
+        by fs [agp32_EX_opc_implies_EX_func] >>
+      fs [EX_ALU_update_def,Rel_def]) >-
+     (PairCases_on `p` >> rw [Run_def,dfn'LoadMEMByte_def,incPC_def] >>
+      `opc ai = 5w` by fs [ag32_Decode_LoadMEMByte_opc_5w] >>
+      `(s''.EX.EX_func = 9w) \/ (s''.EX.EX_func = 12w) \/ (s''.EX.EX_func = 13w) \/
+      (s''.EX.EX_func = 14w) \/ (s''.EX.EX_func = 15w)`
+        by fs [agp32_EX_opc_implies_EX_func] >>
+      fs [EX_ALU_update_def,Rel_def]) >-
+     (PairCases_on `p` >> rw [Run_def,dfn'LoadUpperConstant_def,incPC_def] >>
+      `opc ai = 14w` by fs [ag32_Decode_LoadUpperConstant_opc_14w] >>
+      `(s''.EX.EX_func = 9w) \/ (s''.EX.EX_func = 12w) \/ (s''.EX.EX_func = 13w) \/
+      (s''.EX.EX_func = 14w) \/ (s''.EX.EX_func = 15w)`
+        by fs [agp32_EX_opc_implies_EX_func] >>
+      fs [EX_ALU_update_def,Rel_def]) >-
+     (PairCases_on `p` >> rw [Run_def,dfn'Normal_def,norm_def,incPC_def] >>
+      `opc ai = 0w` by fs [ag32_Decode_Normal_opc_0w] >>
+      pairarg_tac >> fs [] >>
+      Cases_on `p0 = fAdd` >-
+       (fs [ALU_def] >> rw [] >>
+        `func ai = 0w` by fs [ag32_Decode_Normal_fAdd_func_0w] >> fs [] >>
+        rw [EX_ALU_update_def,ALU_correct_carry_lem,WORD_LS,word_add_def,w2n_w2w] >>
+        fs [ALU_input1_def,ALU_input2_def] >>
+        `(dataA ai = ri2word p2 ai) /\ (dataB ai = ri2word p3 ai)`
+          by fs [ag32_Decode_Normal_dataA,ag32_Decode_Normal_dataB] >>
+        rw [] >> METIS_TAC [w2n_add_MOD_itself]) >>
+      Cases_on `p0 = fAddWithCarry` >-
+       (fs [ALU_def] >> rw [] >>
+        `func ai = 1w` by fs [ag32_Decode_Normal_fAddWithCarry_func_1w] >> fs [] >>
+        rw [EX_ALU_update_def,ALU_correct_carry_lem,WORD_LS,word_add_def,w2n_w2w] >>
+        fs [ALU_input1_def,ALU_input2_def] >>
+        `(dataA ai = ri2word p2 ai) /\ (dataB ai = ri2word p3 ai)`
+          by fs [ag32_Decode_Normal_dataA,ag32_Decode_Normal_dataB] >-
+         (`s.EX.EX_carry_flag` by fs [Rel_def] >>
+          rw [v2w_single_1w,ALU_correct_v2w_carry33_lem] >>
+          METIS_TAC [w2n_add_MOD_itself_1]) >>
+        `~s.EX.EX_carry_flag` by fs [Rel_def] >>
+        rw [v2w_single_0w,ALU_correct_v2w_carry33_lem] >>
+        METIS_TAC [w2n_add_MOD_itself]) >>
+      fs [] >> rename1 `(v,ai')` >>
+      `ai'.CarryFlag = ai.CarryFlag` by (fs [ALU_def] >> Cases_on `p0` >> fs [] >> rw []) >>
+      `(func ai <> 0w) /\ (func ai <> 1w)` by fs [ag32_Decode_Normal_func_not_0w_1w] >>
+      fs [EX_ALU_update_def,Rel_def] >>
+      Cases_on_word_value `(agp32 fext fbits (SUC t)).EX.EX_func` >> fs []) >-
+     (PairCases_on `p` >> rw [Run_def,dfn'Out_def,norm_def,incPC_def] >>
+      `opc ai = 6w` by fs [ag32_Decode_Out_opc_6w] >>
+      pairarg_tac >> fs [] >>
+      Cases_on `p0 = fAdd` >-
+       (fs [ALU_def] >> rw [] >>
+        `func ai = 0w` by fs [ag32_Decode_Out_fAdd_func_0w] >> fs [] >>
+        rw [EX_ALU_update_def,ALU_correct_carry_lem,WORD_LS,word_add_def,w2n_w2w] >>
+        fs [ALU_input1_def,ALU_input2_def] >>
+        `(dataA ai = ri2word p2 ai) /\ (dataB ai = ri2word p3 ai)`
+          by fs [ag32_Decode_Out_dataA,ag32_Decode_Out_dataB] >>
+        rw [] >> METIS_TAC [w2n_add_MOD_itself]) >>
+      Cases_on `p0 = fAddWithCarry` >-
+       (fs [ALU_def] >> rw [] >>
+        `func ai = 1w` by fs [ag32_Decode_Out_fAddWithCarry_func_1w] >> fs [] >>
+        rw [EX_ALU_update_def,ALU_correct_carry_lem,WORD_LS,word_add_def,w2n_w2w] >>
+        fs [ALU_input1_def,ALU_input2_def] >>
+        `(dataA ai = ri2word p2 ai) /\ (dataB ai = ri2word p3 ai)`
+          by fs [ag32_Decode_Out_dataA,ag32_Decode_Out_dataB] >-
+         (`s.EX.EX_carry_flag` by fs [Rel_def] >>
+          rw [v2w_single_1w,ALU_correct_v2w_carry33_lem] >>
+          METIS_TAC [w2n_add_MOD_itself_1]) >>
+        `~s.EX.EX_carry_flag` by fs [Rel_def] >>
+        rw [v2w_single_0w,ALU_correct_v2w_carry33_lem] >>
+        METIS_TAC [w2n_add_MOD_itself]) >>
+      fs [] >> rename1 `(v,ai')` >>
+      `ai'.CarryFlag = ai.CarryFlag` by (fs [ALU_def] >> Cases_on `p0` >> fs [] >> rw []) >>
+      `(func ai <> 0w) /\ (func ai <> 1w)` by fs [ag32_Decode_Out_func_not_0w_1w] >>
+      fs [EX_ALU_update_def,Rel_def] >>
+      Cases_on_word_value `(agp32 fext fbits (SUC t)).EX.EX_func` >> fs []) >-
+     (rw [Run_def] >>
+      `opc ai = 15w` by fs [ag32_Decode_ReservedInstr_opc_15w] >>
+      `(s''.EX.EX_func = 9w) \/ (s''.EX.EX_func = 12w) \/ (s''.EX.EX_func = 13w) \/
+      (s''.EX.EX_func = 14w) \/ (s''.EX.EX_func = 15w)`
+        by fs [agp32_EX_opc_implies_EX_func] >>
+      fs [EX_ALU_update_def,Rel_def]) >-
+     (PairCases_on `p` >> rw [Run_def,dfn'Shift_def,incPC_def] >>
+      `opc ai = 1w` by fs [ag32_Decode_Shift_opc_1w] >>
+      `(s''.EX.EX_func = 9w) \/ (s''.EX.EX_func = 12w) \/ (s''.EX.EX_func = 13w) \/
+      (s''.EX.EX_func = 14w) \/ (s''.EX.EX_func = 15w)`
+        by fs [agp32_EX_opc_implies_EX_func] >>
+      fs [EX_ALU_update_def,Rel_def]) >-
+     (PairCases_on `p` >> rw [Run_def,dfn'StoreMEM_def,incPC_def] >>
+      `opc ai = 2w` by fs [ag32_Decode_StoreMEM_opc_2w] >>
+      `(s''.EX.EX_func = 9w) \/ (s''.EX.EX_func = 12w) \/ (s''.EX.EX_func = 13w) \/
+      (s''.EX.EX_func = 14w) \/ (s''.EX.EX_func = 15w)`
+        by fs [agp32_EX_opc_implies_EX_func] >>
+      fs [EX_ALU_update_def,Rel_def]) >>
+    PairCases_on `p` >> rw [Run_def,dfn'StoreMEMByte_def,incPC_def] >>
+    `opc ai = 3w` by fs [ag32_Decode_StoreMEMByte_opc_3w] >>
+    `(s''.EX.EX_func = 9w) \/ (s''.EX.EX_func = 12w) \/ (s''.EX.EX_func = 13w) \/
+    (s''.EX.EX_func = 14w) \/ (s''.EX.EX_func = 15w)`
+      by fs [agp32_EX_opc_implies_EX_func] >>
+    fs [EX_ALU_update_def,Rel_def]) >>
+  `I' (3,SUC t) = I' (3,t)` by fs [is_sch_def,is_sch_disable_def] >>
+  `~s''.ID.ID_EX_write_enable` by fs [enable_stg_def,Abbr `s`] >>
+  rw [EX_ALU_update_def] >>
+  fs [Rel_def,EX_Rel_def]
 QED
 
 val _ = export_theory ();
